foo.v
@@ -1,0 +1,44 @@
+Axiom bu : nat = bool.
+
+Definition g : bool -> nat :=
+  match bu in _ = b return b -> nat with
+  | eq_refl => fun x => x
+  end. 
+
+Definition f : nat -> bool :=
+  match bu in _ = b return nat -> b with
+  | eq_refl => fun x => x
+  end.
+
+Definition fg (x : nat) : g (f x) = x :=
+  match bu as bu return (match bu in _ = b return b -> nat with
+                   | eq_refl => fun x => x
+                   end) ((match bu in _ = b return nat -> b with
+                       | eq_refl => fun x => x
+                       end) x) = x with
+  | eq_refl => eq_refl
+  end.
+
+Goal False.
+pose proof (fg 0) as H1.
+pose proof (fg 1) as H2.
+pose proof (fg 2) as H3.
+destruct (f _);
+destruct (f _); destruct (f _).
+- rewrite H2 in H1.
+discriminate.
+- rewrite H2 in H1.
+discriminate.
+- rewrite H3 in H1.
+discriminate.
+- rewrite H2 in H3.
+discriminate.
+- rewrite H2 in H3.
+discriminate.
+- rewrite H3 in H1.
+discriminate.
+- rewrite H2 in H1.
+discriminate.
+- rewrite H2 in H1.
+discriminate.
+Qed.
