theories/erase_type_in_indexes.v
@@ -1,0 +1,255 @@
+Require Import MetaCoq.Template.All.
+From MetaCoq.PCUIC Require Import PCUICReflect.
+From MetaCoq.PCUIC Require Import TemplateToPCUIC.
+Import MCMonadNotation.
+Require Import utilities.
+Require Import List.
+Require Import String.
+Import ListNotations.
+Unset MetaCoq Strict Unquote Universe Mode.
+
+(** Description of the transformation erase_type_in_indexes
+
+A non-mutual inductive
+
+I (P1 : T1) ... (Pk : Tk) : Type -> ... -> Type := (with l types)
+| C1 x11 ... x1m : I P1 ... Pk TyC11 ... TyC1l
+...
+| Cn xn1 ... xnm : I P1 ... Pk TyCn1 ... TyCnl.
+
+where all the TyCijs are closed types
+
+is transformed into an inductive 
+I' (P1 : T1) ... (Pk : Tk) : Type :=
+| C1' x11 ... x1m : I' P1 ... Pk
+...
+| Cn' xn1 ... xnm : I' P1 ... Pk.
+
+We simply erase the type information *)
+
+
+(** Step 1: find the number of indexes of type Type or Set in the inductive *)
+
+Fixpoint skipn_prods (n : nat) (t : term) :=
+  match n with
+    | 0 => t
+    | S n => 
+      match t with
+       | tProd na Ty u => skipn_prods n u
+       | _ => t
+      end
+    end.
+
+Fixpoint nb_args_codomain_type_or_set (t: term) : option nat :=
+  match t with
+    | tProd _ Ty u => 
+      match Ty with
+        | tSort s => if Universe.is_prop s then None else
+          match (nb_args_codomain_type_or_set u) with
+           | Some x => Some (S x)
+           | None => None
+          end
+        | _ => None
+        end
+    | _ => Some 0
+end.
+
+Definition find_nbr_arity mind : option nat :=
+  let (x, y) := (mind.(ind_npars), (List.hd default_body mind.(ind_bodies)))
+                    in 
+                   let Ty_ind := y.(ind_type) in
+                   nb_args_codomain_type_or_set (skipn_prods x Ty_ind).
+
+(** Step 2: look at the codomain of constructors and remove from npars to npars + nbarity 
+arguments of return type *)
+
+Fixpoint keep_firstn_args (t : term) (npars : nat) :=
+  match t with
+    | tProd Na Ty u => tProd Na Ty (keep_firstn_args u npars) 
+    | tApp u l => tApp u (List.firstn npars l)
+    | _ => t
+  end.
+
+Definition create_oind_transformed oind npars id : one_inductive_entry :=
+  {| 
+    mind_entry_typename := id;
+    mind_entry_arity := <% Type %> ;
+    mind_entry_consnames := List.map (fun x => String.append x "'") oind.(mind_entry_consnames);
+    mind_entry_lc := List.map (fun x => keep_firstn_args x npars) oind.(mind_entry_lc) ;
+   |}.
+
+Definition create_mind_transformed mind id : mutual_inductive_entry :=
+  let npars := List.length mind.(mind_entry_params) in
+  {| 
+    mind_entry_record := mind.(mind_entry_record);
+    mind_entry_finite := mind.(mind_entry_finite);
+    mind_entry_params := mind.(mind_entry_params);
+    mind_entry_inds := List.map (fun x => create_oind_transformed x npars id) 
+      mind.(mind_entry_inds);
+    mind_entry_universes := mind.(mind_entry_universes); 
+    mind_entry_template := mind.(mind_entry_template); 
+    mind_entry_variance := mind.(mind_entry_variance);
+    mind_entry_private := mind.(mind_entry_private);
+  |}. 
+
+
+(* Step 3 : building the Coq function from the initial type to the result type *)
+
+Definition get_name_constructors_first_oind mind :=
+  match hd_error (mind_entry_inds mind) with
+    | None => tmFail "cannot get any inductives in this mutual inductive entry"%bs
+    | Some y => tmReturn (mind_entry_consnames y)
+  end.
+
+Definition first_inductive (kn : kername) :=
+{| inductive_mind := kn ; inductive_ind := 0 |}.
+
+Fixpoint gen_names_tys (nb_arity : nat) :=
+  match nb_arity with
+    | 0 => [mkNamed "t"%bs]
+    | S n => mkNamed "Ty"%bs :: gen_names_tys n
+  end.
+
+Fixpoint build_branchs (lcnames : list (list aname)) (lc' : list term) (lpars : list term) :=
+  match lcnames, lc' with
+    | l :: ls, t :: ts  => {| bcontext := l ; bbody := tApp t (List.map (lift (Datatypes.length l) 0) lpars) |} :: 
+      build_branchs ls ts lpars 
+    | _, _ => []
+  end.
+
+Fixpoint get_n_constructors (n : nat) (i : inductive) := 
+  match n with
+   | 0 => []
+   | S n' => tConstruct i n' [] :: get_n_constructors n' i
+  end.
+
+(* build a lambda binding variables of type Type with suitable names *)
+Fixpoint mkLambda_ty (t : term) (n : nat) (n0 : nat)  :=
+  match n with
+    | 0 => t
+    | S n' => let s := string_of_nat (n'-n) in
+      tLambda (mkNamed (String.append "A" s)) (tSort fresh_universe) (mkLambda_ty t n' n0)
+  end.
+   
+
+Definition build_match_traduction (kn kn' : kername) (lpars : list term) 
+  (nb_arity : nat)
+  (lcnames : list (list aname)) (* list of names for arguments of constructors of the initial type *)
+  (lc' : list term) (* list of constructors of the transformed type *) :=
+    tCase {| ci_ind := first_inductive kn ; ci_npar := Datatypes.length lpars;
+      ci_relevance := Relevant |} 
+          {| puinst := [] ; pparams := lpars ; pcontext := gen_names_tys nb_arity;
+      preturn := tApp (tInd (first_inductive kn') []) lpars |}
+          (tRel 0) (build_branchs lcnames lc' lpars).
+
+
+Fixpoint names_of_prods (t : term) :=
+  match t with
+    | tProd Na _ u => Na :: names_of_prods u
+    | _ => []
+  end.
+
+Definition names_for_args_constructor_first_oind mind :=
+  match hd_error (mind_entry_inds mind) with
+    | None => []
+    | Some y => List.map (fun x => names_of_prods x) (mind_entry_lc y)
+  end. 
+
+Definition build_traduction (kn kn' : kername) (lpars : list term) 
+  (nb_arity : nat)
+  (lcnames : list (list aname)) (* list of names for arguments of constructors of the initial type *)
+  (lc' : list term) := 
+  let n := Datatypes.length lpars in
+  mkLambda_ty (tLambda (mkNamed "x"%bs) 
+    (tApp (tInd {| inductive_mind := kn ; inductive_ind := 0 |} []) lpars) 
+        (build_match_traduction kn kn' lpars nb_arity lcnames lc')) n n.
+
+(** Step 4 : final transformation *) Print tmMkInductive. 
+
+Definition get_curmodpath := curmodpath <- tmCurrentModPath tt ;; tmReturn curmodpath.
+
+Definition erase_type_in_indexes (tm : term) curmodpath :=
+  match tm with
+    | tInd ({| inductive_mind := kn ; inductive_ind := 0 |}) u =>
+        decl <- tmQuoteInductive (inductive_mind  ({| inductive_mind := kn ; inductive_ind := 0 |})) ;;
+        fresh <- tmFreshName (String.append kn.2 "'"%bs) ;;
+      match find_nbr_arity decl with
+        | None => 
+            tmFail "wrong argument given to the transformation"%bs 
+        | Some 0 => 
+            tmPrint "the transformation does nothing here: the type is not dependent or not handled"%bs
+        | Some (S n) =>
+                let indu_entry := mind_body_to_entry decl in 
+                let npars := List.length indu_entry.(mind_entry_params) in
+                let lcnames := names_for_args_constructor_first_oind indu_entry in
+                let nb_constructors := Datatypes.length lcnames in
+                let lpars := Rel_list npars 0 in
+                tmMkInductive true (create_mind_transformed indu_entry fresh);;
+                let lc' := get_n_constructors nb_constructors ({| inductive_mind :=                 
+                (curmodpath, fresh) ; inductive_ind := 0 |}) in
+               tmReturn (build_traduction kn (curmodpath, (String.append kn.2 "'"%bs)) lpars
+              (S n) lcnames lc')
+        end
+    | _ => tmPrint tm ;; tmFail " is not an inductive"%bs
+end.
+
+
+(** Tests **)
+
+Inductive door : Type := Left | Right.
+
+Inductive DOORS : Type -> Type :=
+| IsOpen : door -> DOORS bool
+| Toggle : door -> DOORS unit.
+
+MetaCoq Run (erase_type_in_indexes <% DOORS %>). 
+Print DOORS'.
+
+Inductive test : Type -> Type -> Type :=
+| test1 : bool -> test (list nat) (bool).
+ MetaCoq Run (erase_type_in_indexes <% test %>).
+Print test'.
+
+Inductive test_parameter (A B : Type) : Type -> Type :=
+| c1 : bool -> door -> test_parameter A B unit.
+MetaCoq Run (erase_type_in_indexes <% test_parameter %>). 
+Print test_parameter'.
+
+Check (nat + (bool + unit))%type.
+Check ((nat + bool) + unit)%type.
+
+(* Step 3: Generation of the transformation function *)
+
+(* Definition transfo1 {A : Type} (d : DOORS A) : DOORS' :=
+    match d with
+      | IsOpen d => IsOpen' d
+      | Toggle d => Toggle' d
+    end.
+
+MetaCoq Quote Recursively Definition transfo1_reif_rec := transfo1.
+
+Print transfo1_reif_rec.
+
+Definition transfo2 {A B : Type} (t : test A B) :=
+  match t with
+    | test1 b => test1' b
+  end.
+MetaCoq Quote Recursively Definition transfo2_reif_rec := transfo2.
+
+Print transfo2_reif_rec.
+
+Definition transfo3 (A B : Type) (C : Type) (t : test_parameter A B C) :=
+  match t with
+    | c1 b d => c1' A B b d
+  end.
+MetaCoq Quote Recursively Definition transfo3_reif_rec := transfo3.
+ *)
+
+
+      
+           
+
+
+
+
+
